erasure/theories/Typed/Annotations.v
@@ -3,7 +3,7 @@ From MetaCoq.Erasure.Typed Require Import ExAst.
 From MetaCoq.Erasure.Typed Require Import Transform.
 From MetaCoq.Erasure.Typed Require Import ResultMonad.
 From MetaCoq.Erasure Require Import ELiftSubst.
-From MetaCoq.Template Require Import utils.
+From MetaCoq.Utils Require Import utils.
 
 Module Ex := ExAst.
 
