erasure/theories/Typed/Transform.v
@@ -1,4 +1,4 @@
-From MetaCoq.Template Require Import utils.
+From MetaCoq.Utils Require Import utils.
 From MetaCoq.Erasure.Typed Require Import ExAst.
 From MetaCoq.Erasure.Typed Require Import ResultMonad.
 From MetaCoq.Erasure.Typed Require Import WcbvEvalAux.
